prove the leader half of lemma_FollowerInfo_Message_Invariant_Induction

ironfleet/src/Dafny/Distributed/Protocol/ZooKeeper/PerformamceProof/BasicInvariants.dfy
@@ -29,6 +29,23 @@ import opened Zookeeper_Performance_Definitions
 import opened ZooKeeper_TimestampedDistributedSystem
 
 
+predicate Basic_Invariants(config:Config, tls:TLS_State) {
+    && DS_Config_Invariant(config, tls)
+    && ZK_Config_Invariant(config, tls)
+    && Leader_QueuedPackets_Invariant(config, tls)
+}
+
+
+lemma lemma_Basic_Invariants(config:Config, tlb:seq<TLS_State>, f:int) 
+    requires SeqIsUnique(config);
+    requires ValidTLSBehavior(config, tlb, f)
+    ensures forall i | 0 <= i < |tlb| :: Basic_Invariants(config, tlb[i]) 
+{
+    lemma_DS_Config_Invariant_Proof(config, tlb, f);
+    lemma_ZK_Config_Invariant_Proof(config, tlb, f);
+    lemma_Leader_QueuedPackets_Invariant_Proof(config, tlb, f);
+}
+
 
 /*****************************************************************************************
 /                                   DSConfigInvariant                                    *
@@ -43,6 +60,7 @@ predicate DS_Config_Invariant(config:Config, tls:TLS_State) {
     && (forall i | 0 <= i < |config| :: 
             i == if tls.t_servers[config[i]].v.FollowerPeer? then tls.t_servers[config[i]].v.follower.my_id else tls.t_servers[config[i]].v.leader.my_id
     )
+    && tls.t_environment.config == config
 }
 
 lemma lemma_DS_Config_Invariant_Proof(config:Config, tlb:seq<TLS_State>, f:int)
@@ -102,4 +120,90 @@ lemma lemma_ZK_Config_Invariant_Proof(config:Config, tlb:seq<TLS_State>, f:int)
         i := i + 1;
     }
 }
+
+
+/*****************************************************************************************
+/                               Facts about the environment                              *
+*****************************************************************************************/
+
+
+/* SentPackets set is monotone increasing */
+predicate SentPacketsSet_Monotone(tls:TLS_State, tls':TLS_State, ep:EndPoint, ios:seq<TZKIo>) 
+    requires ep in tls.t_servers
+    requires TLS_NextOneServer(tls, tls', ep, ios)
+    requires LEnvironment_Next(tls.t_environment, tls'.t_environment)
+{
+    var new_sent := IosSeqToSentSet(ios);
+    tls'.t_environment.sentPackets == tls.t_environment.sentPackets + new_sent
+}
+
+
+lemma lemma_SentPacketsSet_Monotone_Induction(config:Config, tls:TLS_State, tls':TLS_State)
+    requires TLS_Next(tls, tls')
+    requires Basic_Invariants(config, tls) && Basic_Invariants(config, tls')
+    ensures forall ep, ios | ep in tls.t_servers && TLS_Next(tls, tls') && TLS_NextOneServer(tls, tls', ep, ios)
+    :: SentPacketsSet_Monotone(tls, tls', ep, ios)
+{
+    // TODO
+    assume false;
+}
+
+
+
+/*****************************************************************************************
+/                                 Facts about the leader                                 *
+*****************************************************************************************/
+
+
+/* QueuedPackets for a LearnerHandler only contains the approriate messages */
+predicate QueuedPackets_Only_Contains_LeaderMessages(q: seq<ZKMessage>) {
+    forall msg | msg in q ::
+        || msg.SyncTRUNC?
+        || msg.SyncSNAP?
+        || msg.SyncDIFF?
+        || msg.Commit?
+}
+
+lemma lemma_LearnerHandler_QueuedPackets_Induction(s:LearnerHandler, s':LearnerHandler, g:LeaderGlobals, g':LeaderGlobals, ios:seq<ZKIo>) 
+    requires LearnerHandlerNext(s, s', g, g', ios);
+    requires QueuedPackets_Only_Contains_LeaderMessages(s.queuedPackets);
+    ensures QueuedPackets_Only_Contains_LeaderMessages(s'.queuedPackets);
+{}
+
+/* QueuedPackets for a LearnerHandler only contains the approriate messages */
+predicate Leader_QueuedPackets_Invariant(config:Config, tls:TLS_State) {
+    forall ep | ep in tls.t_servers ::
+        tls.t_servers[ep].v.LeaderPeer? ==> (
+            forall lh | lh in tls.t_servers[ep].v.leader.handlers
+            :: QueuedPackets_Only_Contains_LeaderMessages(lh.queuedPackets)
+    )
+}
+
+lemma lemma_Leader_QueuedPackets_Invariant_Proof(config:Config, tlb:seq<TLS_State>, f:int)
+    requires SeqIsUnique(config);
+    requires ValidTLSBehavior(config, tlb, f)
+    ensures forall i | 0 <= i < |tlb| :: Leader_QueuedPackets_Invariant(config, tlb[i]) 
+{
+    var handlers := tlb[0].t_servers[config[0]].v.leader.handlers;
+    assert forall i | 1 <= i < |config| :: LearnerHandlerInit(handlers[i-1], 0, i, config);
+    forall i | 0 <= i < |handlers| 
+    ensures LearnerHandlerInit(handlers[i], 0, i+1, config)
+    { 
+        var k := i + 1;
+        assert 1 <= k < |config|;
+        assert LearnerHandlerInit(handlers[k-1], 0, k, config);
+    }
+    var i := 0;
+    while i < |tlb| - 1 
+        decreases |tlb| - i
+        invariant 0 <= i < |tlb|
+        invariant forall k | 0 <= k <= i :: Leader_QueuedPackets_Invariant(config, tlb[k])
+    {
+        var tls, tls' := tlb[i], tlb[i+1];
+        assert Leader_QueuedPackets_Invariant(config, tls');
+        i := i + 1;
+    }
+}
+
+
 }
