ironfleet/src/Dafny/Distributed/Protocol/ZooKeeper/PerformamceProof/ProofEmptyDiff.dfy
@@ -12,6 +12,7 @@ include "../Leader.dfy"
 include "../LearnerHandler.dfy"
 include "Definitions.dfy"
 include "PerformancePredicates.dfy"
+include "BasicInvariants.dfy"
 
 
 module Zookeeper_PerformanceProof {
@@ -28,6 +29,7 @@ import opened ZooKeeper_LearnerHandler
 import opened Zookeeper_Performance_Definitions
 import opened ZooKeeper_TimestampedDistributedSystem
 import opened Zookeeper_PerformancePredicates
+import opened Zookeeper_BasicInvariants
 
 
 /* Main theorem */
@@ -42,21 +44,92 @@ lemma theorem_ZK_Performance_Guarantee(config:Config, tlb:seq<TLS_State>, f:int)
 }
 
 
-predicate FollowerInfo_Message_Guarantee(tls:TLS_State)
-{
-    var perf_formula := SendFI;
-    forall ep | ep in tls.t_environment.channels :: (
-        forall pkt | pkt in tls.t_environment.channels[ep].channel
-        :: pkt.msg.ts == perf_formula
+
+/*****************************************************************************************
+*                                FollowerInit_Invariant                                  *
+*****************************************************************************************/
+
+
+predicate FollowerInit_Invariant(tls:TLS_State){
+    forall ep | ep in tls.t_servers :: (
+        && tls.t_servers[ep].v.FollowerPeer? 
+        && tls.t_servers[ep].v.follower.state == F_HANDSHAKE_A
+        ==> 
+        && tls.t_servers[ep].ts == TimeZero()
     )
 }
 
-lemma lemma_FollowerInfo_Message_Guarantee(config:Config, tlb:seq<TLS_State>, f:int)
-    requires SeqIsUnique(config);
-    requires ValidTLSBehavior(config, tlb, f)
-    requires Performance_Assumption_EmptyDiff(tlb)
-    ensures forall i | 0 <= i < |tlb| :: FollowerInfo_Message_Guarantee(tlb[i])
+lemma lemma_FollowerInit_Invariant_Induction(config:Config, tls:TLS_State, tls':TLS_State)
+    requires TLS_Next(tls, tls')
+    requires Basic_Invariants(config, tls) && Basic_Invariants(config, tls')
+    requires General_LS_Performance_Assumption(tls)
+    // Induction hypothesis
+    requires FollowerInit_Invariant(tls)
+    ensures FollowerInit_Invariant(tls')
+{}
+
+
+
+/*****************************************************************************************
+*                            FollowerInfo_Message_Invariant                              *
+*****************************************************************************************/
+
+
+predicate FollowerInfo_Message_Invariant(tls:TLS_State)
 {
-    assume false;
+    var perf_formula := SendFI;
+    forall pkt | pkt in tls.t_environment.sentPackets && pkt.msg.v.FollowerInfo?
+    :: pkt.msg.ts == perf_formula
 }
+
+
+lemma lemma_FollowerInfo_Message_Invariant_Induction(config:Config, tls:TLS_State, tls':TLS_State)
+    requires TLS_Next(tls, tls')
+    requires Basic_Invariants(config, tls) && Basic_Invariants(config, tls')
+    requires General_LS_Performance_Assumption(tls)
+    // Induction hypothesis
+    requires FollowerInfo_Message_Invariant(tls)
+    ensures FollowerInfo_Message_Invariant(tls')
+{
+    var actor, tios :| actor in tls.t_servers && TLS_NextOneServer(tls, tls', actor, tios);
+    var ls, ls', ios := UntagLS_State(tls), UntagLS_State(tls'), UntagLIoOpSeq(tios);
+    assert LS_NextOneServer(ls, ls', actor, ios);
+    if ls.servers[actor].FollowerPeer? {
+        // TODO
+        assume FollowerInfo_Message_Invariant(tls');
+    } else {
+        /* No new FollowerInfo messages get sent, so nothing to worry */
+        var s, s' := ls.servers[actor].leader, ls'.servers[actor].leader;
+        assert LeaderNext(s, s', ios);
+        if s.state == L_STARTING {
+            if |ios| > 0 {
+                var h, h' := s.handlers[s.nextHandlerToStep], s'.handlers[s.nextHandlerToStep];
+                var g, g' := s.globals, s'.globals;
+                assert LearnerHandlerNext(h, h', g, g', ios);
+                match h.state 
+                case LH_HANDSHAKE_A => 
+                    assert GetEpochToPropose(h, h', g, g', ios);
+                    assert forall io | io in ios && io.LIoOpSend? :: !io.s.msg.FollowerInfo?;
+                case LH_HANDSHAKE_B => 
+                    assert WaitForEpochAck(h, h', g, g', ios);
+                    assert forall io | io in ios && io.LIoOpSend? :: !io.s.msg.FollowerInfo?;
+                case LH_PREP_SYNC => 
+                    assert PrepareSync(h, h', g, g', ios);
+                    assert |ios| == 0;
+                case LH_SYNC => 
+                    /* Note that this case uses Leader_QueuedPackets_Invariant to make sure
+                     that there are no FollowerInfo sneaking inside queued packets */
+                    assert ZooKeeper_LearnerHandler.DoSync(h, h', g, g', ios);
+                    assert forall io | io in ios && io.LIoOpSend? :: !io.s.msg.FollowerInfo?;
+                case LH_PROCESS_ACK => 
+                    assert ZooKeeper_LearnerHandler.ProcessAck(h, h', g, g', ios);
+                    assert forall io | io in ios && io.LIoOpSend? :: !io.s.msg.FollowerInfo?;
+                case LH_RUNNING => assert |ios| == 0;
+                case LH_ERROR => assert |ios| == 0;
+            }
+        }
+        assert FollowerInfo_Message_Invariant(tls');  
+    }
+}
+
 }
